Backup

dorami/P_entry.s
@@ -1,0 +1,3 @@
+P_entry_from_F:
+    li t0, 0x9B9898989D1E
+    csrw pmpcfg0, t0
