dorami/Sally_Port.s
@@ -1,0 +1,10 @@
+sallyport_entry:
+    csrci mstatus, 0x08
+
+    li t0, 0x8001FFD4
+    csrw mtvec, t0
+
+    li t0, 0x9B989D989D1E
+    csrw pmpcfg0, t0
+
+    jal zero, -0x10816
