dorami/exit_firmware.s
@@ -1,0 +1,1 @@
+csrw pmpcfg0, 0
