examples/add.s
@@ -1,4 +1,5 @@
 addi a0, a0, 1
-addi a0, a0, 1
-addi a0, a0, 1
-ret
+sb	 a0, 0(a1)
+jal a0, 0
+nop
+mret
