examples/add.v
@@ -5,6 +5,8 @@ Definition test_add_spec `{!islaG Σ} `{!threadG} : iProp Σ :=
   ∃ (r : addr),
     reg_col sys_regs ∗
     "x10" ↦ᵣ RVal_Bits (BV 64 0) ∗
+    "x1" ↦ᵣ RVal_Bits r ∗
+    ⌜bv_extract 0 1 r = (BV 1 0)⌝ ∗ ⌜bv_extract 1 1 r = (BV 1 0)⌝ ∗
     instr_pre (bv_unsigned r) (
       reg_col sys_regs ∗
       "x10" ↦ᵣ RVal_Bits (BV 64 3) ∗ True
@@ -12,10 +14,12 @@ Definition test_add_spec `{!islaG Σ} `{!threadG} : iProp Σ :=
 Arguments test_add_spec /.
 
 Lemma test_state_iris_fn1 `{!islaG Σ} `{!threadG} :
-  instr 0x0000000010300010 (Some a0) -∗
-  instr 0x0000000010300014 (Some a4) -∗
-  instr_body 0x0000000010300010 test_add_spec.
+  instr 0x0000000010300000 (Some a8) -∗
+  instr_body 0x0000000010300000 test_add_spec.
 Proof.
   iStartProof.
-  repeat liAStep; liShow.
+
+  liARun.
+  Unshelve. all: prepare_sidecond.
+  all: try bv_solve.
 Qed.
