universal_contract/femtokernel.v
@@ -2,78 +2,18 @@ Require Import isla.riscv64.riscv64.
 
 Context `{!islaG Σ} `{!threadG}.
 
-(* reg_col for GPR and PMP? How about other CSR? *)
-Definition Step_pre m (h i mpp: bv 64) : iProp Σ :=
-  arch_pc_reg ↦ᵣ RVal_Bits i ∗ "cur_privilege" ↦ᵣ RVal_Enum m ∗
-  "mtvec" # "bits" ↦ᵣ RVal_Bits h ∗ (∃ c, "mcause" # "bits" ↦ᵣ RVal_Bits c) ∗
-  "mstatus" # "bits" ↦ᵣ RVal_Bits mpp ∗ (∃ c, "mepc" ↦ᵣ RVal_Bits c).
-
-(* Can it be NONE? probably no. *)
-Definition Execution (inst_trace: gmap (bv 64) isla_trace) m (h mpp: bv 64) : iProp Σ :=
-  (∃ (i: bv 64) t, arch_pc_reg ↦ᵣ RVal_Bits i ∗ ⌜inst_trace !! i = Some t⌝) ∗
-  "cur_privilege" ↦ᵣ RVal_Enum m ∗ "mtvec" # "bits" ↦ᵣ RVal_Bits h ∗
-  (∃ c, "mcause" # "bits" ↦ᵣ RVal_Bits c) ∗
-  "mstatus" # "bits" ↦ᵣ RVal_Bits mpp ∗ (∃ c, "mepc" ↦ᵣ RVal_Bits c).
-
-(* Add inst_trace parameter to CSRMod, Trap, and Recover. *)
-Definition CSRMod m : iProp Σ :=
-  (∃ i, arch_pc_reg ↦ᵣ RVal_Bits i) ∗ ⌜m = "Machine"⌝ ∗ "cur_privilege" ↦ᵣ RVal_Enum m ∗
-  (∃ h, "mtvec" # "bits" ↦ᵣ RVal_Bits h) ∗ (∃ c, "mcause" # "bits" ↦ᵣ RVal_Bits c) ∗
-  (∃ ms, "mstatus" # "bits" ↦ᵣ RVal_Bits ms) ∗ (∃ me, "mepc" ↦ᵣ RVal_Bits me).
-
-Definition Trap (h: bv 64) : iProp Σ :=
-  arch_pc_reg ↦ᵣ RVal_Bits h ∗ "cur_privilege" ↦ᵣ RVal_Enum "Machine" ∗
-  "mtvec" # "bits" ↦ᵣ RVal_Bits h ∗ (∃ c, "mcause" # "bits" ↦ᵣ RVal_Bits c) ∗
-  "mstatus" # "bits" ↦ᵣ RVal_Bits (BV 64 0x0000000000000000)  ∗ (∃ c, "mepc" ↦ᵣ RVal_Bits c).
-
-Definition Recover  m (h: bv 64) : iProp Σ :=
-  (∃ i, arch_pc_reg ↦ᵣ RVal_Bits i ∗ "mepc" ↦ᵣ RVal_Bits i) ∗ ⌜m = "Machine" ⌝ ∗
-  "cur_privilege" ↦ᵣ RVal_Enum "User" ∗ "mtvec" # "bits" ↦ᵣ RVal_Bits h ∗
-  (∃ c, "mcause" # "bits" ↦ᵣ RVal_Bits c) ∗
-  "mstatus" # "bits" ↦ᵣ RVal_Bits (BV 64 0x0000000000000000) ∗ (∃ c, "mepc" ↦ᵣ RVal_Bits c).
-
-Definition step_contract :=
-  ∀ inst_trace t m h i mpp,
-  (([∗ map] inst ↦ trace ∈ inst_trace, (instr (bv_unsigned inst) (Some trace)))
-   ∗ ⌜inst_trace !! i = Some t⌝)-∗
-  ((Execution inst_trace m h mpp
-    ∨ CSRMod m
-    ∨ Trap h
-    ∨ Recover m h) -∗ WPasm tnil) -∗
-  (Step_pre m h i mpp -∗ WPasm t).
-
-Definition cycle_precond m h i mpp : iProp Σ :=
-  Step_pre m h i mpp ∗
-  (CSRMod m -∗ WPasm tnil) ∗
-  (Trap h -∗ WPasm tnil) ∗
-  (Recover m h -∗ WPasm tnil).
-
-Definition cycle_contract : iProp Σ :=
-  ∀ m h i mpp,
-  (∃ inst_trace t, ([∗ map] inst ↦ trace ∈ inst_trace, instr (bv_unsigned inst) (Some trace))
-     ∗ ⌜inst_trace !! i = Some t⌝) -∗
-   (cycle_precond m h i mpp) -∗
-   WPasm tnil.
-
-(* Implicit Arg in Hypothesis *)
-Hypothesis valid_step_contract :
-  step_contract.
-
-Lemma valid_cycle_contract : ⊢ cycle_contract.
-Proof.
-  iLöb as "IH".
-  iIntros (m h i mpp) "(%inst_trace & %t & #Hinst_trace & %Hinst) (Hpre & HCSRMod & HTrap & HRecover)".
-  iDestruct "Hpre" as "(Hpc&?&?&?&?&?)".
-  iApply (wp_next_instr i with "[$Hpc] [Hinst_trace]");
-  first iPoseProof (big_sepM_lookup_acc _ _ _ _ Hinst with "[$Hinst_trace]") as "[$ _]".
-  iModIntro.
-  iIntros "Hpc".
-  iApply (valid_step_contract inst_trace t m h i mpp with "[$Hinst_trace //] [HCSRMod HTrap HRecover] [$]").
-  iIntros "[HRes | [HRes | [HRes | HRes]]]".
-  - iDestruct "HRes" as "((%i' & %t' & Hpc & %Hinst')&?&?&?&?&?)".
-    iApply ("IH" with "[$Hinst_trace]"); first by auto.
-    iFrame.
-  - by iApply "HCSRMod".
-  - by iApply "HTrap".
-  - by iApply "HRecover".
+Lemma zgtz : 0 > 0 -> False.
+  lia.
 Qed.
+
+Definition pred_strong1 (n: nat): n > 0 -> nat :=
+  match n with
+  | O => fun pf => match zgtz pf with end
+  | S n' => fun _ => n'
+  end.
+
+Theorem two_gt0 : 2 > 0.
+  lia.
+Qed.
+
+Eval compute in pred_strong1 2 two_gt0.
