universal_contract/universal_contract.v
@@ -1,18 +1,23 @@
 Require Import isla.riscv64.riscv64.
 
-(* reg_col for GPR and PMP? How about other CSR? *)
+(* TODO: reg_col for GPR and PMP? How about other CSR? *)
+(* TODO: list the perm fro mem and inst for the fixed region. *)
+(* TODO: use instr directly instead of instr_table. *)
 Definition MStep_pre `{!islaG Σ} `{!threadG} (h i: bv 64) (entries: list (bv 64 * bv 8)): iProp Σ :=
-  arch_pc_reg ↦ᵣ RVal_Bits i ∗ "cur_privilege" ↦ᵣ RVal_Enum "Machine" ∗
+  arch_pc_reg ↦ᵣ RVal_Bits i ∗ (∃ tbl t, instr_table tbl ∗ ⌜tbl !! i = Some t⌝) ∗ "cur_privilege" ↦ᵣ RVal_Enum "Machine" ∗
   "mtvec" # "bits" ↦ᵣ RVal_Bits h ∗ (∃ mc, "mcause" # "bits" ↦ᵣ RVal_Bits mc) ∗
   (∃ ms, "mstatus" # "bits" ↦ᵣ RVal_Bits ms) ∗ (∃ me, "mepc" ↦ᵣ RVal_Bits me) ∗
   reg_col (pmp_regs entries) ∗ interp_pmp entries "Machine".
 
 (* Can it be NONE? probably no. *)
-Definition PMPHold  `{!islaG Σ} `{!threadG} (inst_trace: gmap (bv 64) isla_trace) (h: bv 64) : iProp Σ :=
-  (∃ (i: bv 64) t, arch_pc_reg ↦ᵣ RVal_Bits i ∗ ⌜inst_trace !! i = Some t⌝) ∗
+(* Two instr at same addr is allowed. *)
+(* TODO: reuse the MStep_pre definition. *)
+Definition PMPHold `{!islaG Σ} `{!threadG} (h: bv 64) (entries: list (bv 64 * bv 8)) : iProp Σ :=
+  (∃ (i: bv 64) tbl t, arch_pc_reg ↦ᵣ RVal_Bits i ∗ instr_table tbl ∗ ⌜tbl !! i = Some t⌝) ∗
   "cur_privilege" ↦ᵣ RVal_Enum "Machine" ∗ "mtvec" # "bits" ↦ᵣ RVal_Bits h ∗
   (∃ mc, "mcause" # "bits" ↦ᵣ RVal_Bits mc) ∗
-  (∃ ms, "mstatus" # "bits" ↦ᵣ RVal_Bits ms) ∗ (∃ me, "mepc" ↦ᵣ RVal_Bits me).
+  (∃ ms, "mstatus" # "bits" ↦ᵣ RVal_Bits ms) ∗ (∃ me, "mepc" ↦ᵣ RVal_Bits me) ∗
+  reg_col (pmp_regs entries) ∗ interp_pmp entries "Machine".
 
 Fixpoint NoPMPWrite (t: isla_trace) : bool :=
   match t with
@@ -22,68 +27,104 @@ Fixpoint NoPMPWrite (t: isla_trace) : bool :=
   | tcases ts => foldr (λ t b, NoPMPWrite t && b) true ts
   end.
 
-(* The instr can also be in pmp_acces *)
-Definition PMPMod : iProp Σ :=
-  (∃ (i: bv 64) t, arch_pc_reg ↦ᵣ RVal_Bits i ∗ instr (bv_unsigned i) (Some t) ∗ ⌜NoPMPWrite t⌝) ∗ "cur_privilege" ↦ᵣ RVal_Enum "Machine" ∗
+Definition PMPMod `{!islaG Σ} `{!threadG} : iProp Σ :=
+  (∃ (i: bv 64) tbl t, arch_pc_reg ↦ᵣ RVal_Bits i ∗ instr_table tbl ∗ ⌜tbl !! i = Some t⌝ ∗ ⌜negb (NoPMPWrite t)⌝) ∗
+  "cur_privilege" ↦ᵣ RVal_Enum "Machine" ∗
   (∃ h, "mtvec" # "bits" ↦ᵣ RVal_Bits h) ∗ (∃ mc, "mcause" # "bits" ↦ᵣ RVal_Bits mc) ∗
-  (∃ ms, "mstatus" # "bits" ↦ᵣ RVal_Bits ms) ∗ (∃ me, "mepc" ↦ᵣ RVal_Bits me).
+  (∃ ms, "mstatus" # "bits" ↦ᵣ RVal_Bits ms) ∗ (∃ me, "mepc" ↦ᵣ RVal_Bits me) ∗
+  (∃ entries, reg_col (pmp_regs entries) ∗ interp_pmp entries "Machine").
 
-Definition MTrap (h: bv 64) : iProp Σ :=
-  arch_pc_reg ↦ᵣ RVal_Bits h ∗ "cur_privilege" ↦ᵣ RVal_Enum "Machine" ∗
+(* Should have the "instr h (Some t)" *)
+Definition MTrap `{!islaG Σ} `{!threadG} (h: bv 64) (entries: list (bv 64 * bv 8)): iProp Σ :=
+  arch_pc_reg ↦ᵣ RVal_Bits h ∗ (∃ tbl t, instr_table tbl ∗ ⌜tbl !! h = Some t⌝) ∗ "cur_privilege" ↦ᵣ RVal_Enum "Machine" ∗
   "mtvec" # "bits" ↦ᵣ RVal_Bits h ∗ (∃ mc, "mcause" # "bits" ↦ᵣ RVal_Bits mc) ∗
-  (∃ ms, "mstatus" # "bits" ↦ᵣ RVal_Bits ms) ∗ (∃ me, "mepc" ↦ᵣ RVal_Bits me).
+  (∃ ms, "mstatus" # "bits" ↦ᵣ RVal_Bits ms) ∗ (∃ me, "mepc" ↦ᵣ RVal_Bits me) ∗
+  reg_col (pmp_regs entries) ∗ interp_pmp entries "Machine".
 
-Definition MRecover (h: bv 64) : iProp Σ :=
-  (∃ i, arch_pc_reg ↦ᵣ RVal_Bits i ∗ "mepc" ↦ᵣ RVal_Bits i) ∗
+(* Should have the "instr i (Some t)" *)
+Definition MRecover `{!islaG Σ} `{!threadG} (h: bv 64) (entries: list (bv 64 * bv 8)): iProp Σ :=
+  (∃ (i: bv 64) tbl t, arch_pc_reg ↦ᵣ RVal_Bits i ∗ instr_table tbl ∗ ⌜tbl !! i = Some t⌝ ∗ "mepc" ↦ᵣ RVal_Bits i) ∗
   "cur_privilege" ↦ᵣ RVal_Enum "User" ∗ "mtvec" # "bits" ↦ᵣ RVal_Bits h ∗
   (∃ c, "mcause" # "bits" ↦ᵣ RVal_Bits c) ∗
-  (∃ ms, "mstatus" # "bits" ↦ᵣ RVal_Bits ms) ∗ (∃ me, "mepc" ↦ᵣ RVal_Bits me).
+  (∃ ms, "mstatus" # "bits" ↦ᵣ RVal_Bits ms) ∗ (∃ me, "mepc" ↦ᵣ RVal_Bits me) ∗
+  reg_col (pmp_regs entries) ∗ interp_pmp entries "User".
 
-Definition step_contract :=
-  ∀ inst_trace t h i,
-  (([∗ map] inst ↦ trace ∈ inst_trace, (instr (bv_unsigned inst) (Some trace)))
-   ∗ ⌜inst_trace !! i = Some t⌝)-∗
-  ((PMPHold inst_trace h
+Definition step_contract `{!islaG Σ} `{!threadG} :=
+  ∀ t h i entries,
+  ((PMPHold h entries
     ∨ PMPMod
-    ∨ MTrap h
-    ∨ MRecover h) -∗ WPasm tnil) -∗
-  (MStep_pre h i -∗ WPasm t).
+    ∨ MTrap h entries
+    ∨ MRecover h entries) -∗ WPasm tnil) -∗
+  (MStep_pre h i entries -∗ WPasm t).
 
-Definition cycle_precond h i : iProp Σ :=
-  MStep_pre h i ∗
-  (PMPMod -∗ WPasm tnil) ∗
-  (MTrap h -∗ WPasm tnil) ∗
-  (MRecover h -∗ WPasm tnil).
+Definition cycle_precond  `{!islaG Σ} `{!threadG} h i entries : iProp Σ :=
+  MStep_pre h i entries ∗
+  ▷(PMPMod -∗ WPasm tnil) ∗
+  ▷(MTrap h entries -∗ WPasm tnil) ∗
+  ▷(MRecover h entries -∗ WPasm tnil).
 
-Definition cycle_contract : iProp Σ :=
-  ∀ h i,
-  (∃ inst_trace t, ([∗ map] inst ↦ trace ∈ inst_trace, instr (bv_unsigned inst) (Some trace))
-     ∗ ⌜inst_trace !! i = Some t⌝) -∗
-   (cycle_precond h i) -∗
+Definition cycle_contract `{!islaG Σ} `{!threadG} : iProp Σ :=
+  ∀ h i entries,
+   (cycle_precond h i entries) -∗
    WPasm tnil.
 
 (* Implicit Arg in Hypothesis *)
+
+Section universal_contract.
+Context `{!islaG Σ} `{!threadG}.
+(* How to remove the context *)
 Hypothesis valid_step_contract :
   step_contract.
 
 Lemma valid_cycle_contract : ⊢ cycle_contract.
-Proof.
+Proof using valid_step_contract.
   iLöb as "IH".
-  iIntros (h i) "(%inst_trace & %t & #Hinst_trace & %Hinst) (Hpre & HCSRMod & HTrap & HRecover)".
-  iDestruct "Hpre" as "(Hpc&?&?&?&?&?)".
-  iApply (wp_next_instr i with "[$Hpc] [Hinst_trace]");
-  first iPoseProof (big_sepM_lookup_acc _ _ _ _ Hinst with "[$Hinst_trace]") as "[$ _]".
+  iIntros (h i entries) "(Hpre & HCSRMod & HTrap & HRecover)".
+  iDestruct "Hpre" as "(Hpc&(%tbl & %t & #Hinstbl & %Hlkins)&?&?&?&?&?&?&?)".
+  Check instr_intro.
+  iPoseProof (instr_intro _ _ _ _ Hlkins with "Hinstbl") as "Hinst".
+  iApply (wp_next_instr i with "[$Hpc] [Hinst]"); first by iFrame.
   iModIntro.
   iIntros "Hpc".
-  iApply (valid_step_contract inst_trace t h i with "[$Hinst_trace //] [HCSRMod HTrap HRecover] [$]").
+  iApply (valid_step_contract t h i entries with "[HCSRMod HTrap HRecover]"); last (iFrame; by auto).
   iIntros "[HRes | [HRes | [HRes | HRes]]]".
-  - iDestruct "HRes" as "((%i' & %t' & Hpc & %Hinst')&?&?&?&?&?)".
-    iApply ("IH" with "[$Hinst_trace]"); first by auto.
-    iFrame.
+  - iDestruct "HRes" as "((%i' & %tbl' & %t' & Hpc' & #Hinstbl' & %Hlkins') &?&?&?&?&?)".
+    iApply "IH". iFrame. by auto.
   - by iApply "HCSRMod".
   - by iApply "HTrap".
   - by iApply "HRecover".
+  Unshelve.
+  apply bv_is_wf.
 Qed.
 
-Parameter firmware_code_range : prod Z Z.
-Parameter firmware_mem_range : prod Z Z.
+Lemma firmware_safety F2P F_start entries :
+  MStep_pre F2P F_start entries -∗
+  (∃ tbl, instr_table tbl ∗ ⌜map_Forall (λ _ t, NoPMPWrite t) tbl⌝) -∗
+  ("cur_privilege" ↦ᵣ RVal_Enum "User" -∗
+   (∀ i, instr i None) ∗ "cur_privilege" ↦ᵣ RVal_Enum "User") -∗ (*TODO: derived from interp_pmp *)
+  (MTrap F2P entries -∗ WPasm tnil) -∗
+  WPasm tnil.
+Proof using  valid_step_contract.
+  iIntros "? #HNoPMPWrite HNoUserInst HTrap".
+  iApply valid_cycle_contract.
+  iFrame.
+  iSplitR.
+  - iIntros "!> ((%i & %tbl & %t & ? & #Hinstbl & %Hinst & %HPMPWrite)&?&?&?&?&?&?)".
+    iDestruct "HNoPMPWrite" as "(%tbl' & Hinstbl' & %Hallinst)".
+    iPoseProof (instr_table_agree with "Hinstbl' Hinstbl") as "->".
+    assert (NoPMPWrite t) by exact (map_Forall_lookup_1 _ _ _ _ Hallinst Hinst).
+    destruct (NoPMPWrite t); by simpl in *.
+  - iIntros "!> ((%i & %tbl & %t & ? & #Hinstbl & %Hinst & Hmepc)&?&?&?&?&?&?&?)".
+    iPoseProof ("HNoUserInst" with "[$]") as "[HNoInst _]".
+    iSpecialize ("HNoInst" $! (bv_unsigned i)).
+    iPoseProof (instr_lookup with "Hinstbl HNoInst") as "%HH".
+    destruct HH as (b & Hb & Hinst').
+    assert (Z_to_bv_checked 64 (bv_unsigned i) = Some i) by (apply Z_to_bv_checked_bv_unsigned).
+    rewrite H0 in Hb.
+    inversion Hb.
+    rewrite -H2 in Hinst'.
+    rewrite Hinst' in Hinst.
+    inversion Hinst.
+Qed.
+
+End universal_contract.
