dorami/instructions/F2P/instrs.v
@@ -1,0 +1,28 @@
+Require Import isla.isla_lang.
+Require Export isla.dorami.instructions.F2P.a0.
+Require Export isla.dorami.instructions.F2P.a4.
+Require Export isla.dorami.instructions.F2P.a8.
+Require Export isla.dorami.instructions.F2P.ac.
+Require Export isla.dorami.instructions.F2P.a10.
+Require Export isla.dorami.instructions.F2P.a14.
+Require Export isla.dorami.instructions.F2P.a18.
+Require Export isla.dorami.instructions.F2P.a1c.
+Require Export isla.dorami.instructions.F2P.a20.
+Require Export isla.dorami.instructions.F2P.a24.
+Require Export isla.dorami.instructions.F2P.a28.
+Require Export isla.dorami.instructions.F2P.a2c.
+
+Definition instr_map := [
+  (0x0%Z, a0 (* csrci mstatus,8 *));
+  (0x4%Z, a4 (* addiw t0,zero,1 *));
+  (0x8%Z, a8 (* slli t0,t0,0x1f *));
+  (0xc%Z, ac (* csrw mtvec,t0 *));
+  (0x10%Z, a10 (* lui t0,0x4dd *));
+  (0x14%Z, a14 (* addiw t0,t0,-945 # 4dcc4f <sallyport_entry+0x4dcc4f> *));
+  (0x18%Z, a18 (* slli t0,t0,0xc *));
+  (0x1c%Z, a1c (* addi t0,t0,-827 *));
+  (0x20%Z, a20 (* slli t0,t0,0xd *));
+  (0x24%Z, a24 (* addi t0,t0,-738 *));
+  (0x28%Z, a28 (* csrw pmpcfg0,t0 *));
+  (0x2c%Z, a2c (* j fffffffffffef7ea *))
+].
