dorami/instructions/Sally_Port/a34.v
@@ -1,0 +1,14 @@
+From isla Require Import opsem.
+
+Definition a34 : isla_trace :=
+  Smt (DeclareConst 0%Z (Ty_BitVec 64%N)) Mk_annot :t:
+  Assume (AExp_Binop (Eq) (AExp_Val (AVal_Var "PC" []) Mk_annot) (AExp_Val (AVal_Bits (BV 64%N 0x80021034%Z)) Mk_annot) Mk_annot) Mk_annot :t:
+  Smt (DeclareConst 1%Z (Ty_BitVec 64%N)) Mk_annot :t:
+  Assume (AExp_Binop (Eq) (AExp_Unop (Extract 2%N 2%N) (AExp_Val (AVal_Var "misa" [Field "bits"]) Mk_annot) Mk_annot) (AExp_Val (AVal_Bits (BV 1%N 0x1%Z)) Mk_annot) Mk_annot) Mk_annot :t:
+  ReadReg "PC" [] (RegVal_Base (Val_Symbolic 0%Z)) Mk_annot :t:
+  Smt (DefineConst 2%Z (Manyop (Bvmanyarith Bvadd) [Val (Val_Symbolic 0%Z) Mk_annot; Val (Val_Bits (BV 64%N 0x4%Z)) Mk_annot] Mk_annot)) Mk_annot :t:
+  Smt (DefineConst 3%Z (Manyop (Bvmanyarith Bvadd) [Val (Val_Symbolic 0%Z) Mk_annot; Val (Val_Bits (BV 64%N 0xfffffffffffdefcc%Z)) Mk_annot] Mk_annot)) Mk_annot :t:
+  Smt (DefineConst 4%Z (Unop (Extract 0%N 0%N) (Binop ((Bvarith Bvlshr)) (Val (Val_Symbolic 3%Z) Mk_annot) (Val (Val_Bits (BV 64%N 0x1%Z)) Mk_annot) Mk_annot) Mk_annot)) Mk_annot :t:
+  WriteReg "PC" [] (RegVal_Base (Val_Symbolic 3%Z)) Mk_annot :t:
+  tnil
+.
