dorami/instructions/Sally_Port/instrs.v
@@ -1,0 +1,32 @@
+Require Import isla.isla_lang.
+Require Export isla.dorami.instructions.Sally_Port.a0.
+Require Export isla.dorami.instructions.Sally_Port.a4.
+Require Export isla.dorami.instructions.Sally_Port.a8.
+Require Export isla.dorami.instructions.Sally_Port.ac.
+Require Export isla.dorami.instructions.Sally_Port.a10.
+Require Export isla.dorami.instructions.Sally_Port.a14.
+Require Export isla.dorami.instructions.Sally_Port.a18.
+Require Export isla.dorami.instructions.Sally_Port.a1c.
+Require Export isla.dorami.instructions.Sally_Port.a20.
+Require Export isla.dorami.instructions.Sally_Port.a24.
+Require Export isla.dorami.instructions.Sally_Port.a28.
+Require Export isla.dorami.instructions.Sally_Port.a2c.
+Require Export isla.dorami.instructions.Sally_Port.a30.
+Require Export isla.dorami.instructions.Sally_Port.a34.
+
+Definition instr_map := [
+  (0x0%Z, a0 (* csrci mstatus,8 *));
+  (0x4%Z, a4 (* lui t0,0x4 *));
+  (0x8%Z, a8 (* addiw t0,t0,1 # 4001 <sallyport_entry+0x4001> *));
+  (0xc%Z, ac (* slli t0,t0,0x11 *));
+  (0x10%Z, a10 (* addi t0,t0,-44 *));
+  (0x14%Z, a14 (* csrw mtvec,t0 *));
+  (0x18%Z, a18 (* lui t0,0x4dd *));
+  (0x1c%Z, a1c (* addiw t0,t0,-945 # 4dcc4f <sallyport_entry+0x4dcc4f> *));
+  (0x20%Z, a20 (* slli t0,t0,0xc *));
+  (0x24%Z, a24 (* addi t0,t0,-827 *));
+  (0x28%Z, a28 (* slli t0,t0,0xd *));
+  (0x2c%Z, a2c (* addi t0,t0,-738 *));
+  (0x30%Z, a30 (* csrw pmpcfg0,t0 *));
+  (0x34%Z, a34 (* j 0xfffffffffffdefcc *))
+].
