dorami/instructions/exit_firmware/instrs.v
@@ -1,0 +1,6 @@
+Require Import isla.isla_lang.
+Require Export isla.dorami.instructions.exit_firmware.a0.
+
+Definition instr_map := [
+  (0x0%Z, a0 (* csrwi pmpcfg0,0 *))
+].
