instructions/add/instrs.v
@@ -1,12 +1,8 @@
 Require Import isla.isla_lang.
-Require Export isla.instructions.add.a0.
 Require Export isla.instructions.add.a4.
 Require Export isla.instructions.add.a8.
-Require Export isla.instructions.add.ac.
 
 Definition instr_map := [
-  (0x0%Z, a0 (* addi a0,a0,1 *));
-  (0x4%Z, a4 (* addi a0,a0,1 *));
-  (0x8%Z, a8 (* addi a0,a0,1 *));
-  (0xc%Z, ac (* ret *))
+  (0x4%Z, a4 (* beq a0,a1,64 *));
+  (0x8%Z, a8 (* jal a0,64 *))
 ].
