instructions/riscv64_test/a8_spec.v
@@ -7,6 +7,58 @@ Lemma a8_spec `{!islaG Σ} `{!threadG} pc:
   ⊢ instr_body pc (sd_spec pc "x11" "x2" (8)).
 Proof.
   iStartProof.
+  do 30 liAStep; liShow.
+  do 10 liAStep; liShow.
+  do 10 liAStep; liShow.
+  do 10 liAStep; liShow.
+  do 10 liAStep; liShow.
+  do 10 liAStep; liShow.
+  liAStep; liShow.
+  liAStep; liShow.
+  liAStep; liShow.
+  liAStep; liShow.
+  liAStep; liShow.
+  liAStep; liShow.
+  liAStep; liShow.
+  liAStep; liShow.
+  simple notypeclasses refine (tac_li_tactic _ _ _ _ _).
+  1:{
+  clear;
+  autounfold with regcol_compute_unfold;
+  repeat match goal with | H := _ |- _  => clearbody H end.
+  remember_regcol.
+  lazymatch goal with
+  | |- LiTactic (regcol_compute_hint ?f ?a) =>
+      (* We first compute the result of f a such that we don't need to
+      create an evor for it, but can use [abstract]. This is important
+      since the [clearbody]s above are otherwise ignored at Qed time,
+      leading to divergence of vm_compute. This means that we run
+      vm_compute twice, but it should be fast anyway. *)
+      let x := eval vm_compute in (f a) in
+      idtac x
+  end.
+  lazymatch goal with
+  | |- LiTactic (regcol_compute_hint ?f ?a) =>
+      (* We first compute the result of f a such that we don't need to
+      create an evor for it, but can use [abstract]. This is important
+      since the [clearbody]s above are otherwise ignored at Qed time,
+      leading to divergence of vm_compute. This means that we run
+      vm_compute twice, but it should be fast anyway. *)
+      let x := eval vm_compute in (f a) in
+      lazymatch x with
+      | Some ?y => apply (regcol_compute_hint_hint y)
+      end
+  end.
+  abstract (vm_compute; exact eq_refl).
+  }
+
+  liTactic.
+  liAStep; liShow.
+  liAStep; liShow.
+  liAStep; liShow.
+  liAStep; liShow.
+  liAStep; liShow.
+  liAStep; liShow.
   repeat liAStep; liShow.
   Unshelve. all: prepare_sidecond.
   all: bv_solve.
