instructions/test/instrs.v
@@ -1,0 +1,6 @@
+Require Import isla.isla_lang.
+Require Export isla.instructions.test.ac.
+
+Definition instr_map := [
+  (0xc%Z, ac (* csrw mtvec,t0 *))
+].
